

Generating function method

Here we present the details of solving the PDEs in the paper with generating functions.

All-cell growth model:

```
In[1]:= ClearAll[G, z, kb, kd, pde]

In[2]:= pde = (kd z - kb - kd) z G'[z] - kb  $\frac{z}{1-z}$  G[z] + kb  $\frac{z}{1-z}$  == 0;

DSolve[pde, G[z], z] // FullSimplify

Out[3]=  $\left\{ \left\{ G[z] \rightarrow \frac{kb + (-1 + z) c_1}{kb + kd - kd z} \right\} \right\}$ 
```

One-end growth model:

```
In[4]:= ClearAll[G, z, pde, γ, Gsum, GsumPrime]

In[5]:= pde = -γ z G'[z] -  $\left( (1 - z) + γ \frac{z}{1-z} \right)$  G[z] + γ  $\frac{z}{1-z}$  == 0;

DSolve[pde, G[z], z] // FullSimplify

Out[6]=  $\left\{ \left\{ G[z] \rightarrow -e^{z/\gamma} (-1 + z) z^{-1/\gamma} \left( c_1 + \int_1^z \frac{e^{-\frac{K[1]}{\gamma}} K[1]^{\frac{1}{\gamma}}}{(-1 + K[1])^2} dK[1] \right) \right\} \right\}$ 
```

$$\text{In[7]:= } G[z_]:= e^{\frac{z}{\gamma}} (1 - z) z^{-1/\gamma} \int_0^z \frac{e^{-\frac{x}{\gamma}} x^{1/\gamma}}{(1 - x)^2} dx;$$

Highlighted[G[z]]

```
Out[8]=  $e^{z/\gamma} (1 - z) z^{-1/\gamma} \int_0^z \frac{e^{-\frac{x}{\gamma}} x^{\frac{1}{\gamma}}}{(1 - x)^2} dx$ 
```

```
In[9]:= Series[G[z], {z, 0, 5}, Assumptions -> γ > 0]

Out[9]=  $\frac{\gamma z}{1 + \gamma} + \frac{2 \gamma z^2}{(1 + \gamma)(1 + 2 \gamma)} + \frac{3 \gamma z^3}{(1 + \gamma)(1 + 2 \gamma)(1 + 3 \gamma)} +$   

 $\frac{4 \gamma z^4}{(1 + \gamma)(1 + 2 \gamma)(1 + 3 \gamma)(1 + 4 \gamma)} + \frac{5 \gamma z^5}{(1 + \gamma)(1 + 2 \gamma)(1 + 3 \gamma)(1 + 4 \gamma)(1 + 5 \gamma)} + O[z]^6$ 
```

(* Check to see that this sum form is the solution to the original PDE *)

```
In[10]:= Gsum = Sum $\left[ \frac{n \gamma^{1-n}}{\text{Pochhammer}[(1 + \gamma) / \gamma, n]} * z^n, \{n, 1, \infty\} \right]$  // FullSimplify;

GsumPrime = D[Gsum, z] // FullSimplify;
```

```
In[12]:= -γ z GsumPrime - ((1 - z) + γ  $\frac{z}{1 - z}$ ) Gsum + γ  $\frac{z}{1 - z}$  // FullSimplify
```

```
Out[12]= 0
```

Two-end growth model:

```
In[13]:= ClearAll[G, z, pde, γ, Gsum, GsumPrime]
```

```
In[14]:= pde = z G'[z] == -( $\frac{2}{\gamma}$  (1 - z) +  $\frac{z}{1 - z}$ ) G[z] +  $\frac{z}{1 - z}$  +  $\frac{1}{1 + \gamma}$  z (1 - z);
```

```
DSolve[pde, G[z], z] // FullSimplify
```

```
Out[15]= 
$$\left\{ \left\{ G[z] \rightarrow -e^{\frac{2z}{\gamma}} (-1 + z) z^{-2/\gamma} \left( c_1 + \int_1^z \frac{e^{-\frac{2K[1]}{\gamma}} K[1]^{2/\gamma} (2 + \gamma + (-2 + K[1]) K[1])}{(1 + \gamma) (-1 + K[1])^2} dK[1] \right) \right\} \right\}$$

```

```
In[16]:= G[z_] := e $\frac{2z}{\gamma}$  (1 - z) z $^{-2/\gamma}$   $\int_0^z \frac{e^{-\frac{2x}{\gamma}} x^{2/\gamma} (x^2 - 2x + 2 + \gamma)}{(1 + \gamma) (1 - x)^2} dx$ ;
```

```
Highlighted[G[z]]
```

```
Out[17]=
```

$$e^{\frac{2z}{\gamma}} (1 - z) z^{-2/\gamma} \int_0^z \frac{e^{-\frac{2x}{\gamma}} x^{2/\gamma} (2 - 2x + x^2 + \gamma)}{(1 - x)^2 (1 + \gamma)} dx$$

```
In[18]:= Series[G[z], {z, 0, 6}, Assumptions → γ > 0]
```

```
Out[18]= 
$$\frac{\gamma z}{1 + \gamma} + \frac{\gamma z^2}{(1 + \gamma)^2} + \frac{3 \gamma z^3}{(1 + \gamma)^2 (2 + 3 \gamma)} + \frac{4 \gamma z^4}{(1 + \gamma)^2 (1 + 2 \gamma) (2 + 3 \gamma)} +$$


$$\frac{10 \gamma z^5}{(1 + \gamma)^2 (1 + 2 \gamma) (2 + 3 \gamma) (2 + 5 \gamma)} + \frac{12 \gamma z^6}{(1 + \gamma)^2 (1 + 2 \gamma) (1 + 3 \gamma) (2 + 3 \gamma) (2 + 5 \gamma)} + O[z]^7$$

```

(* Check to see that this sum form is the solution to the original PDE *)

```
In[19]:= Gsum =  $\frac{\gamma}{1 + \gamma}$  z + Sum[ $\frac{2 + \gamma}{2 (1 + \gamma)}$   $\frac{n (\gamma / 2)^{1-n}}{\text{Pochhammer}[(2 + \gamma) / \gamma, n]}$  * zn, {n, 2, ∞}] // FullSimplify;
```

```
GsumPrime = D[Gsum, z] // FullSimplify;
```

```
In[21]:= z GsumPrime + ( $\frac{2}{\gamma}$  (1 - z) +  $\frac{z}{1 - z}$ ) Gsum -  $\frac{z}{1 - z}$  -  $\frac{1}{1 + \gamma}$  z (1 - z) // FullSimplify
```

```
Out[21]= 0
```

Conditional survival probability:

```
In[22]:= ClearAll[G, z, t, kb, kd, pde, initCond]
```

```
In[23]:= pde = D[G[z, t], t] == - (kb + kd) z D[G[z, t], z] + kd D[G[z, t], z] - (kd / z) G[z, t];
```

$$\text{initCond} = G[z, 0] = \sum_{n=1}^{\infty} z^n;$$

```
In[25]:= sol = DSolve[{pde, initCond}, G, {z, t}]
```

```
Out[25]=
```

$$\left\{ \left\{ G \rightarrow \text{Function}\left[\{z, t\}, \frac{(kb + kd) z}{\left(-1 + e^{kb \left(t - \frac{\text{Log}[kd (-1+z) + kb z]}{kb + kd}\right)} + kd \left(t - \frac{\text{Log}[kd (-1+z) + kb z]}{kb + kd}\right) kb\right) (-kd + kb z + kd z)}\right] \right\} \right\}$$

```
In[26]:= G = sol[[1, 1, 2, 2]] // FullSimplify;
```

```
Highlighted[G]
```

```
Out[27]=
```

$$\frac{(kb + kd) z}{e^{(kb + kd) t} kb + kd - (kb + kd) z}$$

```
In[28]:= SeriesCoefficient[G, {z, 0, n}]
```

```
Out[28]=
```

$$\begin{cases} \left(\frac{kb + kd}{e^{(kb + kd) t} kb + kd} \right)^n & n \geq 1 \\ 0 & \text{True} \end{cases}$$